user 3, session 11481, part 2

diffs-no-failures-no-compiles-clean/3/user-3-session-11481.v
@@ -21,3 +21,25 @@ Unset Search Output Name Only.
 Timeout 1 Print LoadPath.
 Module Exercises (vars: VarsAPI).
 Check vars.read.
+Check vars.write.
+Definition incX : proc unit :=
+  x <- vars.read VarX; _ <- vars.write VarX (x + 1); Ret tt.
+Redirect "/var/folders/5x/1mdbpbjd7012l971fq0zkj2w0000gn/T/coqammdPf"
+Print Ltac Signatures.
+Timeout 1 Print Grammar tactic.
+Add Search Blacklist "Raw" "Proofs".
+Set Search Output Name Only.
+Redirect "/var/folders/5x/1mdbpbjd7012l971fq0zkj2w0000gn/T/coqRwctHg"
+SearchPattern _.
+Remove Search Blacklist "Raw" "Proofs".
+Unset Search Output Name Only.
+Theorem incX_test :
+  proc_spec
+    (fun (_ : unit) state =>
+     {|
+     pre := state = mkState 1 2 3;
+     post := fun r state' => state' = mkState 2 2 3;
+     recovered := fun _ state' => False |}) incX vars.recover vars.abstr.
+Proof.
+(unfold incX).
+step_proc.
